LeanProjeto2/ExemplosSect1.lean
@@ -45,62 +45,62 @@ example (σ τ : FType) : FType := (σ⋆ ⟶ τ)⋆
 -- -------------------------
 
 -- Ex1.4(1). t₁t₂ : τ where t₁ : σ → τ and t₂ : σ
-example (σ τ : FType) (t₁ t₂ : Term) (h1: TypeChecking t₁ (σ ⟶ τ)) (h2 : TypeChecking t₂ σ) : TypeChecking (app t₁ t₂) τ :=
+example (σ τ : FType) (t₁ t₂ : Term) (h1: Term_TypeChecking t₁ (σ ⟶ τ)) (h2 : Term_TypeChecking t₂ σ) : Term_TypeChecking (app t₁ t₂) τ :=
   by
-    exact TypeChecking.tcApp h1 h2
+    exact Term_TypeChecking.tcApp h1 h2
 
 -- Ex1.4(1). tx : τ where t : σ → τ and x : σ
-example (σ τ : FType) (t : Term) (x : string) (h1: TypeChecking t (σ ⟶ τ)) (h2 : TypeChecking (var x) σ) : TypeChecking (app t (var x)) τ :=
+example (σ τ : FType) (t : Term) (x : String) (h1: Term_TypeChecking t (σ ⟶ τ)) (h2 : Term_TypeChecking (var x) σ) : Term_TypeChecking (app t (var x)) τ :=
   by
-   exact TypeChecking.tcApp h1 h2
+   exact Term_TypeChecking.tcApp h1 h2
 
 -- Ex1.4(2). (pt)(tx) : ρ where p: (σ → τ) → τ → ρ, t : σ → τ and x : σ
-example (σ τ ρ : FType) (p t : Term) (x: string) (h1 : TypeChecking p ((σ⟶τ)⟶τ⟶ρ)) (h2: TypeChecking t (σ ⟶ τ)) (h3 : TypeChecking (var x) σ) : TypeChecking (app (app p t) (app t (var x))) ρ :=
+example (σ τ ρ : FType) (p t : Term) (x: String) (h1 : Term_TypeChecking p ((σ⟶τ)⟶τ⟶ρ)) (h2: Term_TypeChecking t (σ ⟶ τ)) (h3 : Term_TypeChecking (var x) σ) : Term_TypeChecking (app (app p t) (app t (var x))) ρ :=
   by
-    have H1 := TypeChecking.tcApp h1 h2
-    have H2 := TypeChecking.tcApp h2 h3
-    exact TypeChecking.tcApp H1 H2
+    have H1 := Term_TypeChecking.tcApp h1 h2
+    have H2 := Term_TypeChecking.tcApp h2 h3
+    exact Term_TypeChecking.tcApp H1 H2
 
 -- Ex1.4(3) - Π₁_{σ,τ} x : τ ⟶ σ where Π₁ : σ ⟶ τ ⟶ σ and x : σ
-example (σ τ : FType) (t : Term) (x : string)
-    (h1 : TypeChecking (var x) σ)
-    (h2 : TypeChecking Π₁ (σ ⟶ τ ⟶ σ)) : TypeChecking (app Π₁ (var x)) (τ ⟶ σ) :=
+example (σ τ : FType) (t : Term) (x : String)
+    (h1 : Term_TypeChecking (var x) σ)
+    (h2 : Term_TypeChecking Π₁ (σ ⟶ τ ⟶ σ)) : Term_TypeChecking (app Π₁ (var x)) (τ ⟶ σ) :=
   by
-    exact TypeChecking.tcApp h2 h1
+    exact Term_TypeChecking.tcApp h2 h1
 
 
 -- Ex1.4(4) - (Σ₁_{σ,τ,ρ} q)t : ρ ⟶ τ where Σ₁ : (σ ⟶ τ ⟶ ρ) ⟶ (σ ⟶ τ) ⟶ σ ⟶ ρ and t : σ ⟶ τ and x : σ
 example (σ τ ρ : FType) (q t : Term)
-    (ht : TypeChecking t (σ ⟶ τ))
-    (hq : TypeChecking q (σ ⟶ τ ⟶ ρ))
-    (hs : TypeChecking Σ₁ ((σ ⟶ (τ ⟶ ρ)) ⟶ ((σ ⟶ τ) ⟶ (σ ⟶ ρ)))) : TypeChecking (app (app Σ₁ q) t) (σ ⟶ ρ) :=
+    (ht : Term_TypeChecking t (σ ⟶ τ))
+    (hq : Term_TypeChecking q (σ ⟶ τ ⟶ ρ))
+    (hs : Term_TypeChecking Σ₁ ((σ ⟶ (τ ⟶ ρ)) ⟶ ((σ ⟶ τ) ⟶ (σ ⟶ ρ)))) : Term_TypeChecking (app (app Σ₁ q) t) (σ ⟶ ρ) :=
   by
-    have H1 := TypeChecking.tcApp hs hq
-    exact TypeChecking.tcApp H1 ht
+    have H1 := Term_TypeChecking.tcApp hs hq
+    exact Term_TypeChecking.tcApp H1 ht
 
 -- Ex1.4(5) -
-example (σ τ : FType) (t : Term) (x: string)
-    (ht : TypeChecking t (σ ⟶ τ))
-    (hx : TypeChecking (var x) σ)
-    (h_sig : TypeChecking Σ₁ ((σ ⟶ τ ⟶ σ) ⟶ (σ ⟶ τ) ⟶ σ ⟶ σ))
-    (h_pi : TypeChecking Π₁ (σ ⟶ τ ⟶ σ)): TypeChecking (app (app (app Σ₁ Π₁) t) (var x)) σ :=
+example (σ τ : FType) (t : Term) (x: String)
+    (ht : Term_TypeChecking t (σ ⟶ τ))
+    (hx : Term_TypeChecking (var x) σ)
+    (h_sig : Term_TypeChecking Σ₁ ((σ ⟶ τ ⟶ σ) ⟶ (σ ⟶ τ) ⟶ σ ⟶ σ))
+    (h_pi : Term_TypeChecking Π₁ (σ ⟶ τ ⟶ σ)): Term_TypeChecking (app (app (app Σ₁ Π₁) t) (var x)) σ :=
   by
-    have H1 := TypeChecking.tcApp h_sig h_pi
-    have H2 := TypeChecking.tcApp H1 ht
-    exact TypeChecking.tcApp H2 hx
+    have H1 := Term_TypeChecking.tcApp h_sig h_pi
+    have H2 := Term_TypeChecking.tcApp H1 ht
+    exact Term_TypeChecking.tcApp H2 hx
 
 -- Ex1.4(6) -
-example (σ τ : FType) (w : Term) (x: string)
-    (hw : TypeChecking w (σ ⟶ τ⋆))
-    (hx : TypeChecking (var x) σ)
-    (h_sing : TypeChecking 𝔰₁ (σ ⟶ σ⋆))
-    (h_i_un : TypeChecking ind_⋃₁ (σ⋆ ⟶ ((σ ⟶ τ⋆) ⟶ τ⋆)))
-    (h_b_un : TypeChecking ∪₁ (τ⋆ ⟶ (τ⋆ ⟶ τ⋆))) : TypeChecking (app ∪₁ (app (app ind_⋃₁ (app 𝔰₁ (var x))) w)) (τ⋆ ⟶ τ⋆) :=
+example (σ τ : FType) (w : Term) (x: String)
+    (hw : Term_TypeChecking w (σ ⟶ τ⋆))
+    (hx : Term_TypeChecking (var x) σ)
+    (h_sing : Term_TypeChecking 𝔰₁ (σ ⟶ σ⋆))
+    (h_i_un : Term_TypeChecking ind_⋃₁ (σ⋆ ⟶ ((σ ⟶ τ⋆) ⟶ τ⋆)))
+    (h_b_un : Term_TypeChecking ∪₁ (τ⋆ ⟶ (τ⋆ ⟶ τ⋆))) : Term_TypeChecking (app ∪₁ (app (app ind_⋃₁ (app 𝔰₁ (var x))) w)) (τ⋆ ⟶ τ⋆) :=
   by
-    have H1 := TypeChecking.tcApp h_sing hx
-    have H2 := TypeChecking.tcApp h_i_un H1
-    have H3 := TypeChecking.tcApp H2 hw
-    exact TypeChecking.tcApp h_b_un H3
+    have H1 := Term_TypeChecking.tcApp h_sing hx
+    have H2 := Term_TypeChecking.tcApp h_i_un H1
+    have H3 := Term_TypeChecking.tcApp H2 hw
+    exact Term_TypeChecking.tcApp h_b_un H3
 
 
 -- ----------------------------------------------
@@ -117,8 +117,8 @@ example (σ τ : FType) (w : Term) (x: string)
 -- FORMULAS
 -- --------------------
 
-open AtomicFormula
-open BaseFormula
+--open AtomicFormula
+--open BaseFormula
 open Formula
 
 
